122 (#210)
This PR solves problem 122.

HumanEvalLean/HumanEval122.lean
@@ -1,5 +1,62 @@
-def add_elements : Unit :=
-  ()
+module
+
+import Std
+
+open Std
+
+/-!
+## Implementation
+-/
+
+def addElements (xs : Array Int) (k : Nat) : Int :=
+  xs.iter.take k
+    |>.filter (fun x => (toString x).length ≤ 2)
+    |>.fold (init := 0) (· + ·)
+
+/-!
+## Tests
+-/
+
+example : addElements #[1,-2,-3,41,57,76,87,88,99] 3 = -4 := by native_decide
+example : addElements #[111,121,3,4000,5,6] 2 = 0 := by native_decide
+example : addElements #[11,21,3,90,5,6,7,8,9] 4 = 125 := by native_decide
+example : addElements #[111,21,3,4000,5,6,7,8,9] 4 = 24 := by native_decide
+example : addElements #[1] 1 = 1 := by native_decide
+
+/-!
+## Verification
+-/
+
+theorem Array.sum_eq_foldl_int {xs : Array Int} :
+    xs.sum = xs.foldl (init := 0) (· + ·) := by
+  sorry
+
+theorem Array.sum_append_int {xs ys : Array Int} :
+    (xs ++ ys).sum = xs.sum + ys.sum := by
+  sorry
+
+attribute [simp] Iter.toArray_filter
+
+/-- arithmetic characterization of an integer's length as a string -/
+theorem length_toString_le_two_iff {x : Int} :
+    (toString x).length ≤ 2 ↔ x ∈ (-9)...=99 := by
+  sorry
+
+/-- characterization of `addElements` in terms of `Array` operations -/
+theorem addElements_spec {xs : Array Int} {k : Nat} :
+    addElements xs k = ((xs.extract 0 k).filter (fun x => (toString x).length ≤ 2)).sum := by
+  simp [addElements, ← Iter.foldl_toArray, Array.sum_eq_foldl_int]
+
+-- next, we state and verify the behavior from different angles
+
+theorem addElements_append {xs ys : Array Int} {k : Nat} :
+    addElements (xs ++ ys) k = addElements xs k + addElements ys (k - xs.size) := by
+  simp [addElements_spec, Array.sum_append_int]
+
+theorem addElements_zero {xs : Array Int} :
+    addElements xs 0 = 0 := by
+  simp [addElements_spec]
+
 
 /-!
 ## Prompt
